src/AwsCryptographicMaterialProviders/Keyrings/AwsKms/AwsKmsMrkAwareSymmetricRegionDiscoveryKeyring.dfy
@@ -1,0 +1,523 @@
+// Copyright Amazon.com Inc. or its affiliates. All Rights Reserved.
+// SPDX-License-Identifier: Apache-2.0
+
+include "../../Keyring.dfy"
+include "../../Materials.dfy"
+include "../../AlgorithmSuites.dfy"
+include "../../../StandardLibrary/StandardLibrary.dfy"
+include "../../../KMS/KMSUtils.dfy"
+include "../../../KMS/AmazonKeyManagementService.dfy"
+include "../../../KMS/AwsKmsArnParsing.dfy"
+include "../../../Util/UTF8.dfy"
+include "../../../../libraries/src/Collections/Sequences/Seq.dfy"
+include "../../../StandardLibrary/Actions.dfy"
+include "Constants.dfy"
+
+module
+  {:extern "Dafny.Aws.Crypto.MaterialProviders.AwsKmsMrkAwareSymmetricRegionDiscoveryKeyring"}
+  MaterialProviders.AwsKmsMrkAwareSymmetricRegionDiscoveryKeyring
+{
+  import opened StandardLibrary
+  import opened Wrappers
+  import opened UInt = StandardLibrary.UInt
+  import opened AwsKmsArnParsing
+  import opened AmazonKeyManagementService
+  import opened Actions
+  import opened Constants
+  import AlgorithmSuites
+  import Keyring
+  import Materials
+  import opened KMSUtils
+  import UTF8
+
+  datatype DiscoveryFilter = DiscoveryFilter(
+    partition: string,
+    accounts: seq<string>
+  )
+
+  class AwsKmsMrkAwareSymmetricRegionDiscoveryKeyring
+    //= compliance/framework/aws-kms/aws-kms-mrk-aware-symmetric-region-discovery-keyring.txt#2.5
+    //= type=implication
+    //# MUST implement that AWS Encryption SDK Keyring interface (../keyring-
+    //# interface.md#interface)
+    extends Keyring.VerifiableInterface
+  {
+    const client: IAmazonKeyManagementService
+    const discoveryFilter: Option<DiscoveryFilter>
+    const grantTokens: GrantTokens
+    const region: string
+
+    //= compliance/framework/aws-kms/aws-kms-mrk-aware-symmetric-region-discovery-keyring.txt#2.6
+    //= type=implication
+    //# On initialization the caller MUST provide:
+    constructor (
+      //= compliance/framework/aws-kms/aws-kms-mrk-aware-symmetric-region-discovery-keyring.txt#2.6
+      //= type=implication
+      //# However if it can not, then it MUST
+      //# NOT create the client itself.
+      client: IAmazonKeyManagementService,
+      //= compliance/framework/aws-kms/aws-kms-mrk-aware-symmetric-region-discovery-keyring.txt#2.6
+      //= type=exception
+      //# It
+      //# SHOULD obtain this information directly from the client as opposed to
+      //# having an additional parameter.
+      region: string,
+      discoveryFilter: Option<DiscoveryFilter>,
+      grantTokens: GrantTokens
+    )
+      //= compliance/framework/aws-kms/aws-kms-mrk-aware-symmetric-region-discovery-keyring.txt#2.6
+      //= type=implication
+      //# It SHOULD have a Region parameter and
+      //# SHOULD try to identify mismatched configurations.
+      requires ReagionMatch(client, region)
+      ensures
+        && this.client          == client
+        && this.region          == region
+        && this.discoveryFilter == discoveryFilter
+        && this.grantTokens     == grantTokens
+    {
+      this.client          := client;
+      //= compliance/framework/aws-kms/aws-kms-mrk-aware-symmetric-region-discovery-keyring.txt#2.6
+      //# The keyring MUST know what Region the AWS KMS client is in.
+      this.region          := region;
+      this.discoveryFilter := discoveryFilter;
+      this.grantTokens     := grantTokens;
+    }
+
+    method OnEncrypt(
+      input: Crypto.OnEncryptInput
+    )
+      returns (res: Result<Crypto.OnEncryptOutput, string>)
+      //= compliance/framework/aws-kms/aws-kms-mrk-aware-symmetric-region-discovery-keyring.txt#2.7
+      //= type=implication
+      //# This function MUST fail.
+      ensures res.Failure?
+    {
+      return Failure("Encryption is not supported with a Discovery Keyring.");
+    }
+
+    //= compliance/framework/aws-kms/aws-kms-mrk-aware-symmetric-region-discovery-keyring.txt#2.8
+    //= type=implication
+    //# OnDecrypt MUST take decryption materials (structures.md#decryption-
+    //# materials) and a list of encrypted data keys
+    //# (structures.md#encrypted-data-key) as input.
+    method OnDecrypt(
+      input: Crypto.OnDecryptInput
+    )
+      returns (res: Result<Crypto.OnDecryptOutput, string>)
+      ensures res.Success?
+      ==>
+        && Materials.DecryptionMaterialsTransitionIsValid(
+          input.materials,
+          res.value.materials
+        )
+
+      ensures
+        input.materials.plaintextDataKey.Some?
+      ==>
+        && res.Failure?
+
+      ensures
+        && input.materials.plaintextDataKey.None?
+        && res.Success?
+      ==>
+        && res.value.materials.plaintextDataKey.Some?
+        && exists edk: Crypto.EncryptedDataKey, awsKmsKey: string
+        |
+          && edk in input.encryptedDataKeys
+        ::
+          // && edk is EncryptedDataKey
+          //= compliance/framework/aws-kms/aws-kms-mrk-aware-symmetric-region-discovery-keyring.txt#2.8
+          //= type=implication
+          //# *  Its provider ID MUST exactly match the value "aws-kms".
+          && edk.keyProviderId == PROVIDER_ID
+          && DecryptCalledWith(
+          //= compliance/framework/aws-kms/aws-kms-mrk-aware-symmetric-region-discovery-keyring.txt#2.8
+          //= type=implication
+          //# To attempt to decrypt a particular encrypted data key
+          //# (structures.md#encrypted-data-key), OnDecrypt MUST call AWS KMS
+          //# Decrypt (https://docs.aws.amazon.com/kms/latest/APIReference/
+          //# API_Decrypt.html) with the configured AWS KMS client.
+            client,
+            //= compliance/framework/aws-kms/aws-kms-mrk-aware-symmetric-region-discovery-keyring.txt#2.8
+            //= type=implication
+            //# When calling AWS KMS Decrypt
+            //# (https://docs.aws.amazon.com/kms/latest/APIReference/
+            //# API_Decrypt.html), the keyring MUST call with a request constructed
+            //# as follows:
+            DecryptRequest(
+              awsKmsKey,
+              edk.ciphertext,
+              input.materials.encryptionContext,
+              grantTokens
+            ))
+          //= compliance/framework/aws-kms/aws-kms-mrk-aware-symmetric-region-discovery-keyring.txt#2.8
+          //= type=implication
+          //# Since the response does satisfies these requirements then OnDecrypt
+          //# MUST do the following with the response:
+          //#*  set the plaintext data key on the decryption materials
+          //#   (structures.md#decryption-materials) as the response "Plaintext".
+          && DecryptResult(
+            awsKmsKey,
+            res.value.materials.plaintextDataKey.value)
+          //= compliance/framework/aws-kms/aws-kms-mrk-aware-symmetric-region-discovery-keyring.txt#2.8
+          //= type=implication
+          //# *  The length of the response's "Plaintext" MUST equal the key
+          //# derivation input length (algorithm-suites.md#key-derivation-input-
+          //# length) specified by the algorithm suite (algorithm-suites.md)
+          //# included in the input decryption materials
+          //# (structures.md#decryption-materials).
+          && Materials.DecryptionMaterialsWithPlaintextDataKey(res.value.materials)
+    {
+
+      var materials := input.materials;
+      var encryptedDataKeys := input.encryptedDataKeys;
+      var suite := AlgorithmSuites.GetSuite(input.materials.algorithmSuiteId);
+
+      :- Need(
+        Materials.DecryptionMaterialsWithoutPlaintextDataKey(materials), 
+        "Keyring received decryption materials that already contain a plaintext data key.");
+
+      //= compliance/framework/aws-kms/aws-kms-mrk-aware-symmetric-region-discovery-keyring.txt#2.8
+      //# The set of encrypted data keys MUST first be filtered to match this
+      //# keyring's configuration.
+      var edkFilterTransform : OnDecryptMRKEncryptedDataKeyFilterMap := new OnDecryptMRKEncryptedDataKeyFilterMap(region, discoveryFilter);
+      var edksToAttempt, parts :- Actions.FlatMapWithResult(edkFilterTransform, encryptedDataKeys);
+
+      forall i
+      | 0 <= i < |parts|
+      ensures
+        && edkFilterTransform.Ensures(encryptedDataKeys[i], Success(parts[i]))
+        && 1 >= |parts[i]|
+        && |encryptedDataKeys| == |parts|
+        && edksToAttempt == Seq.Flatten(parts)
+        && |encryptedDataKeys| >= |edksToAttempt|
+        && multiset(parts[i]) <= multiset(edksToAttempt)
+        && multiset(edksToAttempt) <= multiset(Seq.Flatten(parts))
+        && forall helper: AwsKmsEdkHelper
+          | helper in parts[i]
+          ::
+            && helper in edksToAttempt
+            && helper.edk == encryptedDataKeys[i]
+            && helper.arn.resource.resourceType == "key"
+      {
+        if |parts| < |edksToAttempt| {
+          Seq.LemmaFlattenLengthLeMul(parts, 1);
+          Seq.LemmaFlattenAndFlattenReverseAreEquivalent(parts);
+          assert |parts| * 1 >= |Seq.Flatten(parts)|;
+        }
+
+        forall helper: AwsKmsEdkHelper
+        | helper in parts[i]
+        ensures
+          && helper in edksToAttempt
+          && helper.edk == encryptedDataKeys[i]
+          && helper.arn.resource.resourceType == "key"
+        {
+          LemmaMultisetSubMemebership(parts[i], edksToAttempt);
+        }
+      }
+
+      forall helper: AwsKmsEdkHelper
+      | helper in edksToAttempt
+      ensures
+        && helper.edk in encryptedDataKeys
+        && helper.arn.resource.resourceType == "key"
+      {
+        LemmaFlattenMembership(parts, edksToAttempt);
+        assert helper in Seq.Flatten(parts);
+      }
+
+      //= compliance/framework/aws-kms/aws-kms-mrk-aware-symmetric-region-discovery-keyring.txt#2.8
+      //# For each encrypted data key in the filtered set, one at a time, the
+      //# OnDecrypt MUST attempt to decrypt the data key.
+      var decryptAction: DecryptSingleEncryptedDataKey := new DecryptSingleEncryptedDataKey(
+        materials,
+        client,
+        region,
+        grantTokens
+      );
+      //= compliance/framework/aws-kms/aws-kms-mrk-aware-symmetric-region-discovery-keyring.txt#2.8
+      //# If the response does not satisfies these requirements then an error
+      //# is collected and the next encrypted data key in the filtered set MUST
+      //# be attempted.
+      var outcome := Actions.ReduceToSuccess(
+        decryptAction,
+        edksToAttempt
+      );
+
+      return match outcome {
+        case Success(mat) =>
+          assert exists helper: AwsKmsEdkHelper
+          | helper in edksToAttempt
+          ::
+            && helper.edk in encryptedDataKeys
+            && helper.arn.resource.resourceType == "key"
+            && decryptAction.Ensures(helper, Success(mat));
+
+          Success(Crypto.OnDecryptOutput(materials := mat))
+        //= compliance/framework/aws-kms/aws-kms-mrk-aware-symmetric-region-discovery-keyring.txt#2.8
+        //# If OnDecrypt fails to successfully decrypt any encrypted data key
+        //# (structures.md#encrypted-data-key), then it MUST yield an error that
+        //# includes all collected errors.
+        case Failure(errors) =>
+          if |errors| == 0 then
+            Failure("Unable to decrypt data key: No Encrypted Data Keys found to match.")
+          else
+            var concatString := (s, a) => a + "\n" + s;
+            var error := Seq.FoldRight(
+              concatString,
+              errors,
+              "Unable to decrypt data key:\n"
+            );
+            Failure(error)
+      };
+    }
+  }
+
+  class OnDecryptMRKEncryptedDataKeyFilterMap
+    extends ActionWithResult<
+      Crypto.EncryptedDataKey,
+      seq<AwsKmsEdkHelper>,
+      string
+    >
+  {
+    const region: string
+    const discoveryFilter: Option<DiscoveryFilter>
+    constructor(
+      region: string,
+      discoveryFilter: Option<DiscoveryFilter>
+    )
+      ensures
+        && this.region == region
+        && this.discoveryFilter == discoveryFilter
+    {
+      this.region := region;
+      this.discoveryFilter := discoveryFilter;
+    }
+
+    predicate Ensures(
+      edk: Crypto.EncryptedDataKey,
+      res: Result<seq<AwsKmsEdkHelper>, string>
+    ) {
+      && (
+        && res.Success?
+      ==>
+        if |res.value| == 1 then
+          && var h := res.value[0];
+          && h.edk.keyProviderId == PROVIDER_ID
+          && h.edk == edk
+          && h.arn.resource.resourceType == "key"
+          && DiscoveryMatch(h.arn, discoveryFilter, region)
+        else
+          && |res.value| == 0
+      )
+    }
+
+    method Invoke(edk: Crypto.EncryptedDataKey
+    )
+      returns (res: Result<seq<AwsKmsEdkHelper>, string>)
+      ensures Ensures(edk, res)
+    {
+
+      if edk.keyProviderId != PROVIDER_ID {
+        return Success([]);
+      }
+
+      // The Keyring produces UTF8 providerInfo.
+      // If an `aws-kms` encrypted data key's providerInfo is not UTF8
+      // this is an error, not simply an EDK to filter out.
+      :- Need(UTF8.ValidUTF8Seq(edk.keyProviderInfo), "Invalid AWS KMS encoding, provider info is not UTF8.");
+
+      var keyId :- UTF8.Decode(edk.keyProviderInfo);
+      var arn :- ParseAwsKmsArn(keyId);
+
+      //= compliance/framework/aws-kms/aws-kms-mrk-aware-symmetric-region-discovery-keyring.txt#2.8
+      //# *  The provider info MUST be a valid AWS KMS ARN (aws-kms-key-
+      //# arn.md#a-valid-aws-kms-arn) with a resource type of "key" or
+      //# OnDecrypt MUST fail.
+      :- Need(arn.resource.resourceType == "key", "Only AWS KMS Keys supported");
+
+      if !DiscoveryMatch(arn, discoveryFilter, region) {
+        return Success([]);
+      }
+
+      return Success([
+        AwsKmsEdkHelper(edk, arn)
+      ]);
+    }
+  }
+
+  class DecryptSingleEncryptedDataKey
+    extends ActionWithResult<
+      AwsKmsEdkHelper,
+      Materials.SealedDecryptionMaterials,
+      string>
+  {
+    const materials: Materials.DecryptionMaterialsPendingPlaintextDataKey
+    const client: IAmazonKeyManagementService
+    const region : string
+    const grantTokens: GrantTokens
+
+    constructor(
+      materials: Materials.DecryptionMaterialsPendingPlaintextDataKey,
+      client: IAmazonKeyManagementService,
+      region : string,
+      grantTokens: GrantTokens
+    )
+      ensures
+      && this.materials == materials
+      && this.client == client
+      && this.region == region
+      && this.grantTokens == grantTokens
+    {
+      this.materials := materials;
+      this.client := client;
+      this.region := region;
+      this.grantTokens := grantTokens;
+    }
+
+    predicate Ensures(
+      helper: AwsKmsEdkHelper,
+      res: Result<Materials.SealedDecryptionMaterials, string>
+    ) {
+        res.Success?
+      ==>
+        && Materials.DecryptionMaterialsTransitionIsValid(materials, res.value)
+        && var awsKmsKey := ToStringForRegion(helper.arn, region);
+        && DecryptCalledWith(
+          client,
+          DecryptRequest(
+            awsKmsKey,
+            helper.edk.ciphertext,
+            materials.encryptionContext,
+            grantTokens
+          )
+        )
+        && DecryptResult(awsKmsKey, res.value.plaintextDataKey.value)
+    }
+
+    method Invoke(
+      helper: AwsKmsEdkHelper
+    )
+      returns (res: Result<Materials.SealedDecryptionMaterials, string>)
+      ensures Ensures(helper, res)
+    {
+
+      var awsKmsKey := ToStringForRegion(helper.arn, region);
+
+      var decryptRequest := KMSUtils.DecryptRequest(
+        awsKmsKey,
+        helper.edk.ciphertext,
+        materials.encryptionContext,
+        grantTokens
+      );
+
+      var decryptResponse :- KMSUtils.Decrypt(client, decryptRequest);
+
+      //= compliance/framework/aws-kms/aws-kms-mrk-aware-symmetric-region-discovery-keyring.txt#2.8
+      //# *  The "KeyId" field in the response MUST equal the requested "KeyId"
+      :- Need(
+        && decryptResponse.keyID == awsKmsKey
+        , "Invalid response from KMS Decrypt");
+
+      var result :-  Materials.DecryptionMaterialsAddDataKey(materials, decryptResponse.plaintext);
+      return Success(result);
+    }
+  }
+
+  function method ToStringForRegion(
+    arn: AwsKmsArn,
+    region: string
+  ): (res: string) {
+    if IsMultiRegionAwsKmsArn(arn) then
+      //= compliance/framework/aws-kms/aws-kms-mrk-aware-symmetric-region-discovery-keyring.txt#2.8
+      //# *  "KeyId": If the provider info's resource type is "key" and its
+      //# resource is a multi-Region key then a new ARN MUST be created
+      //# where the region part MUST equal the AWS KMS client region and
+      //# every other part MUST equal the provider info.
+      arn.ToArnString(Some(region))
+    else
+      //= compliance/framework/aws-kms/aws-kms-mrk-aware-symmetric-region-discovery-keyring.txt#2.8
+      //# Otherwise it MUST
+      //# be the provider info.
+      arn.ToString()
+  }
+
+  function method DiscoveryMatch(
+    arn: AwsKmsArn,
+    discoveryFilter: Option<DiscoveryFilter>,
+    region:string
+  ):
+    (res: bool)
+    ensures
+      && discoveryFilter.Some?
+      && res
+    ==>
+      //= compliance/framework/aws-kms/aws-kms-mrk-aware-symmetric-region-discovery-keyring.txt#2.8
+      //= type=implication
+      //# *  If a discovery filter is configured, its partition and the
+      //# provider info partition MUST match.
+      && discoveryFilter.value.partition == arn.partition
+      //= compliance/framework/aws-kms/aws-kms-mrk-aware-symmetric-region-discovery-keyring.txt#2.8
+      //= type=implication
+      //# *  If a discovery filter is configured, its set of accounts MUST
+      //# contain the provider info account.
+      && discoveryFilter.value.accounts <= [arn.account]
+    //= compliance/framework/aws-kms/aws-kms-mrk-aware-symmetric-region-discovery-keyring.txt#2.8
+    //= type=implication
+    //# *  If the provider info is not identified as a multi-Region key (aws-
+    //# kms-key-arn.md#identifying-an-aws-kms-multi-region-key), then the
+    //# provider info's Region MUST match the AWS KMS client region.
+    ensures
+      && !IsMultiRegionAwsKmsArn(arn)
+      && res
+    ==>
+      arn.region == region
+  {
+    && match discoveryFilter {
+      case Some(filter) =>
+        && filter.partition == arn.partition
+        && filter.accounts <= [arn.account]
+      case None() => true
+    }
+    && if !IsMultiRegionAwsKmsArn(arn) then
+      region == arn.region
+    else
+      true
+  }
+
+  lemma LemmaMultisetSubMemebership<T>(a: seq<T>, b: seq<T>)
+    requires multiset(a) <= multiset(b)
+    ensures forall i | i in a :: i in b
+  {
+    if |a| == 0 {
+    } else {
+      assert multiset([Seq.First(a)]) <= multiset(b);
+      assert Seq.First(a) in b;
+      assert a == [Seq.First(a)] + a[1..];
+      LemmaMultisetSubMemebership(a[1..], b);
+    }
+  }
+
+  lemma LemmaFlattenMembership<T>(parts: seq<seq<T>>, flat: seq<T>)
+    requires Seq.Flatten(parts) == flat
+    ensures forall index
+    | 0 <= index < |parts|
+    :: multiset(parts[index]) <= multiset(flat)
+    ensures multiset(Seq.Flatten(parts)) == multiset(flat)
+    ensures forall part | part in parts
+    :: (forall i | i in part :: i in flat)
+    ensures forall i | i in flat
+    :: (exists part | part in parts :: i in part)
+  {
+    if |parts| == 0 {
+    } else {
+      assert multiset(Seq.First(parts)) <= multiset(flat);
+      assert parts == [Seq.First(parts)] + parts[1..];
+      assert flat ==  Seq.First(parts) + Seq.Flatten(parts[1..]);
+      LemmaFlattenMembership(parts[1..], Seq.Flatten(parts[1..]));
+    }
+  }
+
+}
